Adds Search Implementation

Treap.dfy
@@ -4,12 +4,56 @@ class Treap {
   var root: TreapNode?
   var prioritySet: set<int> //Keeps track of what priority was used.
 
+  constructor () {
+    this.root := null;
+  }
+
+  ghost predicate Valid()
+    reads this, root, if root != null then root.repr else {}
+  {
+    root != null ==> root.Valid()
+  }
+
+
   method Build(values: array<int>) {}
   method Insert(value: int) {}
-  method Delete(value: int) {}
-  method Search(value: int) {}
+  method Delete(value: int) {
+  }
 
-  method RotateLeft(node: TreapNode) {}
+  // Initial search entry point
+  method Search(value: int) returns (node: TreapNode?)
+    requires Valid()
+  {
+    if(root == null){
+      return null;
+    }
+    var ans := SearchNode(root, value);
+    return ans;
+  }
+
+  // Recursive search using nodes
+  method SearchNode(currRoot: TreapNode, value: int)
+    returns (node: TreapNode?)
+    requires currRoot.Valid()
+    ensures if node != null then node.key == value else true
+    decreases currRoot.repr
+  {
+    if (currRoot.key == value) {
+      return currRoot;
+    }
+    if (currRoot.key < value && currRoot.right != null) {
+      var ans := SearchNode(currRoot.right, value);
+      return ans;
+    }
+    if (currRoot.key > value && currRoot.left!= null) {
+      var ans := SearchNode(currRoot.left, value);
+      return ans;
+    }
+    return null;
+  }
+
+  method RotateLeft(node: TreapNode) {
+  }
   method RotateRight(node: TreapNode) {}
 
   // To allow for different implementation of RNG
@@ -17,4 +61,11 @@ class Treap {
   method RandomNumberGenerator() returns (priority: int) {
     return -1;
   }
+}
+
+// Used for testing
+method Main() {
+  var treap := new Treap();
+  var result := treap.RandomNumberGenerator();
+  print (result);
 }
