TreapNode.dfy
@@ -3,11 +3,33 @@ class TreapNode {
   const priority: int
   var left: TreapNode?
   var right: TreapNode?
+  var parent: TreapNode?
 
-  constructor TreapNode(key:int, priority:int) {
+  // Needed to ensure no cycles in between nodes
+  ghost var repr: set<TreapNode>
+
+  ghost predicate Valid()
+    reads this, repr
+  {
+    && this in repr
+    && ( left != null ==>
+         && left in repr
+         && this !in left.repr
+         && left.repr <= repr
+         && left.Valid())
+    && ( right != null ==>
+         && right in repr
+         && this !in right.repr
+         && right.repr <= repr
+         && right.Valid())
+  }
+
+  constructor (key:int, priority:int) {
     this.key := key;
-    this.priority:= priority;
+    this.priority := priority;
     this.left := null;
-    this.right:= null;
+    this.right := null;
+    this.parent := null;
+    repr := {this};
   }
 }
